#physics #electricity #potentialenergy
- electrostatic force is a conservative force: $$ F_{x}=-\frac{\textup{d}U}{\textup{d}x}\Rightarrow F_{e}=-\frac{\textup{d}U_{e}}{\textup{d}r}\Rightarrow\textup{d}U_{e}=-\vec{F}_{e}\cdot\textup{d}\vec{r}\Rightarrow\int\textup{d}U_{e}=-\int\vec{F}_{e}\cdot\textup{d}\vec{r}\Rightarrow\Delta U_{e}=-\int\vec{F}_{e}\cdot\textup{d}\vec{r} $$
	- continuing on with it: $$\vec{E}=\frac{\vec{F}_{e}}{q}\Rightarrow\vec{F}_{e}=q\vec{E}\Rightarrow \Delta U_{e}=-\int^{B}_{A} q\vec{E}\cdot\textup{d}\vec{r}\Rightarrow \Delta U_{e}=-q\int^{B}_{A}\vec{E}\cdot\textup{d}\vec{r}=-q\int^{B}_{A}E\cos\theta\:\textup{d}r $$
	- this determines the change in electric potential energy experienced by a charged particle which has moved from point A to point B in an electric field
	- change in potential does not depend on the path taken from point A to point B
		- moving a positive charge vertically upward in a constant downward electric field makes its electric potential greater than 0 (accelerates in the opposite direction of the electric field): $\Delta U_{e}> 0$  
		- moving a negative charge vertically downward in a constant downward electric field makes its electric potential greater than 0 (accelerates in the direction of the electric field): $\Delta U_{e}>0$ 
	- moving a charge opposite the direction of an electric field will cause: $$\Rightarrow \Delta U_{e}=-q\int^{B}_{A} E\cos(180\degree)\:\textup{d}r=-q\int^{B}_{A}E(-1)\:\textup{d}r=q\int^{B}_{A}E\:\textup{d}r$$
		- the change in PE $(U_{e})$ of a positive charge to be positive
		- the change in PE $(U_{e})$ of a negative charge to be negative
- electric field $(E)$ : force experienced  by a small, positive test charge: $$ \vec{E}= \frac{\vec{F}_{e}}{q} $$
- electric potential $(V)$ : energy experienced by a small positive test charge: $$ V = \frac{U_{e}}{q}\Rightarrow \frac{J}{C}=V, \:\textup{volts} $$
	- a scalar attribute of a vector electric field (no direction)
	- $\Delta V$ is the difference in the electric potential between two points: $$ \Delta V=V_{f}-V_{i}=V_{B}-V_{A}\Rightarrow \Delta V = \frac{\Delta U_{e}}{q}= \frac{-q\int^{B}_{A}\vec{E}\cdot\:\textup{d}\vec{r}}{q}\Rightarrow\Delta V =-\int^{B}_{A}\vec{E}\cdot\textup{d}\vec{r}$$
		- $V_{i}$ is normally zero, so: $$ \Delta V = -\int^{B}_{A} \vec{E}\cdot\textup{d}\vec{r}\Rightarrow\textup{d}V=-\vec{E}\cdot\textup{d}\vec{r}\Rightarrow E_{r}=-\frac{\textup{d}V}{\textup{d}r}$$
	- 
